
\section{Theory}
\subsection{Set the scene}

Input: $x_0\in \R^m $

Latents: $x_t\in\R^m,z\in\R^d, t=1\hdots T$

\subsection{Diffusion process}
\begin{gather}
x_0\rightarrow x_1 \rightarrow  \hdots \rightarrow x_T \rightarrow z \\
q(x_t|x_{t-1})=\N(x_t;x_{t-1},\beta_t I),\beta_t\in\R,\quad  t=1\hdots T\\
\end{gather}

\subsection{Encoder}
\begin{gather}
    q(z|x_T)=\N(z;\mu_\phi (x_T), \sigma^2_\phi (x_T) I), \quad \sigma^2_\phi(x_T)\in \R^d\\
p(z)=\N(z;0,I)\\
\end{gather}

\subsection{Tools}
\begin{gather}
    q(x_t|x_0)=\N(x_t;x_0,\bar\beta_t),\quad \bar\beta_t=\sum_{i=1}^t\\
    q(x_t|x_{t-1}) =q(x_t|x_{t-1}, x_0)=\frac{q(x_{t-1}|x_t, x_0)q(x_t|x_0)}{q(x_{t-1}| x_0)}\\
    q(x_{1:T},z|x_0)=q(z|x_T)\prod_{t=1}^T q(x_t|x_{t-1})\\
    p(x_{0:T},z) = p(z) p(x_T|z)\prod_{t=1}^T p(x_{t-1}|x_t)
 \end{gather}
 \begin{gather}
     q(x_{t-1}|x_t,x_0)=
     \N\left(x_{t-1}; 
     \frac{
     {x_t\bar\beta_{t-1}}
     +{x_0\beta_t}
     }{\bar\beta_{t}}
     , 
     \frac{\beta_t \bar\beta_{t-1}}{\bar\beta_{t}}
     \right), \quad t=2\hdots T
 \end{gather}


\subsection{Loss}

\begin{align}
    L(x_0) &=
    -
    \E_{q(x_1|x_0)}\left[
    \log p(x_0|x_1)\right]
    +
    \sum_{t=2}^T \E_{q(x_t|x_0)}\left[D_{KL}\big(q(x_{t-1}|x_t, x_0)||p(x_{t-1}|x_t)\big)\right]\\
    %
    &\qquad
    -
    \E_{q(x_T,z|x_0)}\left[
    \log p(x_T|z)\right]
    +
    \E_{q(x_T|x_0)}\left[
    D_{KL}\big(q(z|x_T)||p(z)\big)\right]
\end{align}


\subsection{Decoder}
\begin{gather}
p(x_{t-1}|x_t)
=\N\left(
x_{t-1};
%mean
\mu_\theta(x_t,t),
%variance
\frac{\beta_t \bar\beta_{t-1}}{\bar\beta_{t}}
\right),
\quad t=2\hdots T
\\
%
p(x_0|x_1)=Beta(a_\theta(x_1),b_\theta(x_1))\\
%
p(x_T|z)=\N\left(x_T;\mu_\theta(z,T+1),\bar\beta_T\right)
\end{gather}

\subsection{KL divergences}
\begin{gather}
D_{KL}\big(q(z|x_T)||p(z)\big)
=
\frac{1}{2}\left(
\log \frac{1}{\prod_{i=1}^d\sigma^2_\phi(x_T)[i]}
-d
+
\sum_{i=1}^d \frac{1}{\sigma^2_\phi(x_T)[i]}
+
\mu_\phi(x_T)^T \sigma^2_\phi(x_T)^{-1} I \mu_\phi(x_T)
\right)\\
%
D_{KL}\big(q(x_{t-1}|x_t, x_0)||p(x_{t-1}|x_t)\big)
=
\frac{\sqrt{\bar\beta_t}}{2\bar\beta_{t-1}}
\norm{
\epsilon
     -\epsilon_\theta(x_t,t)
     }^2,\qquad x_t=x_0 + \sqrt{\bar\beta_t}\epsilon, \quad \epsilon\sim\N(0,I)\\
\end{gather}

\subsection{Likelihoods}
\begin{align}
    \log p(x_T|z)
    &= \log\N(x_T;\mu_\theta(z,T+1), \bar\beta_T)
    \\
    &=\log \left\{(2\pi)^{-k/2}\det(\bar\beta_TI)^{-1/2}\exp\left(-\frac{1}{2}(x_T-\mu_\theta(z,T+1))^T(\bar\beta_TI)^{-1}(x_T-\mu_\theta(z,T+1))\right)\right\}
    \\
    &=
    -\frac{1}{2 \bar\beta_T}(x_T-\mu_\theta(z,T+1))^2
    \\
\end{align}
\begin{align}
    \log p(x_0|x_1)
    &=
    (a_\theta(x_1)-1)^T\log x_0
    +
    (b_\theta(x_1)-1)^T\log (1-x_0)
    \\
    &\qquad\qquad
    +\sum_{i=1}^m\bigg\{
    \log\Gamma\big\{a_\theta(x_1)[i] + b_\theta(x_1)[i]\big\}
    -
    \log \Gamma\big\{a_\theta(x_1)[i]\big\}
    -
    \log\Gamma\big\{ b_\theta(x_1)[i]\big\}
    \bigg\}
\end{align}